Refactored out code related to building the WFG from a state.

Completeness.v
@@ -1,3 +1,4 @@
+(* begin hide *)
 Require Import ResourceDependency.
 Require Import DependencyState.
 Require Import DependencyStateImpl.
@@ -9,151 +10,66 @@ Require Import Graphs.FGraphs.
 Require Import Coq.Lists.SetoidList.
 Require Import MapUtil SetUtil.
 Require Import Bool.
+(* end hide *)
 
-(** The projection module takes a map I and generates a list of pairs
-    each holds a resource and a task. *)
-Module I_Proj := Project.Project Map_RES Set_TID.
-Definition impedes_edges : impedes -> list (resource * tid) := I_Proj.edges.
+(**
+  The cornerstone of the proof of completeness is to note that
+  the WFG obtained from the a totally deadlocked state has an
+  important property: all nodes (tasks) have outgoing
+  edges. A finite graph with such property is known include a cycle.
+  The final step of the proof is to show that the WFG of the
+  totally deadlocked state is a subgraph of the WFG obtained from the
+  deadlocked state. As we know that a cycle in a subraph is also in the
+  graph that induces it, we get that the cycle exists in the deadlocked
+  state.
+*)
 
-(** By using lemma [Project.edges_spec], we get that any pair
-    in [impedes_edges] is an [IEdge] (aka impedes relation). *)
-Lemma impedes_edges_spec:
-  forall r t d,
-  List.In (r,t) (impedes_edges (get_impedes d)) <-> IEdge d r t.
-Proof.
-  intros.
-  unfold IDep.
-  unfold impedes_edges.
-  apply I_Proj.edges_spec.
-  - intros. destruct H, k1, k2.
-    auto.
-  - auto.
-Qed.
+(** * Building the WFG *)
 
-(** Similarly, we project the map I into pairs of tasks and resources. *)
-Module W_Proj := Project.Project Map_TID Set_RES.
-Definition waits_edges : waits -> list (tid * resource) := W_Proj.edges.
-(** By using lemma [Project.edges_spec], we get that any pair
-    in [waits_edges] is a [WEdge] (aka impedes relation). *)
-Lemma waits_edges_spec:
-  forall t r d,
-  List.In (t,r) (waits_edges (get_waits d)) <-> WEdge d t r.
-Proof.
-  intros.
-  unfold waits_edges.
-  unfold WDep.
-  apply W_Proj.edges_spec.
-  - auto.
-  - intros. destruct H, e1, e2.
-    auto.
-Qed.
-
-(** Given the impedes of a dependency state [d], filter the edges
-    matching [r]. *)
-Definition impedes_matching d r := 
-  filter
-  (fun e:(resource*tid)=>
-    let (r', t) := e in
-    if RES.eq_dec r' r then true else false)
-  (impedes_edges (get_impedes d)).
-(** Given a task [t] waiting for resource [r], compute WEdges starting
-    from [t]. The definition uses function [impedes_matching]. *)
-Definition build_edges (d:dependencies) (e:(tid*resource)) : list (tid*tid) :=
-  let (t, r) := e in
-  map (fun e':(resource*tid)=> (t, snd e')) (impedes_matching d r).
-(** For each blocked tasks in the dependency state compute the WEdges
-    using function [build_edges].*)
-Definition build_wfg (d:dependencies) : list (tid*tid) :=
-  flat_map (build_edges d) (waits_edges (get_waits d)).
-(** The first main result is to show that any pair in
-     [build_wfg] is a [WEdge]. The proof uses lemmas
-     [waits_edges_spec] and [impedes_edges_spec]. *)
-Theorem build_wfg_spec:
-  forall d t t',
-  List.In (t,t') (build_wfg d) <-> 
-  (exists (r:resource), WEdge d t r /\ IEdge d r t').
-Proof.
-  intros.
-  unfold build_wfg.
-  rewrite in_flat_map.
-  unfold build_edges in *.
-  split.
-  - intros.
-    (* We have that there exists a (t1, r) in [wait_edges]. *)
-    destruct H as ((t1, r), (Hinw, Hinb)).
-    rewrite waits_edges_spec in Hinw.
-    (* Thus, we have that (t1, r) is a [WEdge]. *)
-    exists r.
-    rewrite in_map_iff in *.
-    destruct Hinb as ((r', t''), (Heq, Hini)).
-    simpl in *.
-    inversion Heq; subst; clear Heq.
-    (* We also know that (r', t') is in [impedes_matching d r]. *)
-    unfold impedes_matching in *.
-    rewrite filter_In in *.
-    destruct Hini as (Hini, Hcnd).
-    remember (Map_RES_Extra.P.F.eq_dec r' r) as b.
-    destruct b.
-    assert (r' = r).
-    destruct a, r', r.
-    auto.
-    subst.
-    clear a Heqb.
-    rewrite impedes_edges_spec in *.
-    intuition.
-    inversion Hcnd.
-  - intros.
-    destruct H as (r, (Hwf, Him)).
-    exists (t, r).
-    rewrite waits_edges_spec.
-    intuition.
-    rewrite in_map_iff.
-    exists (r, t').
-    simpl.
-    intuition.
-    unfold impedes_matching.
-    rewrite filter_In.
-    split.
-    * rewrite impedes_edges_spec.
-      assumption.
-    * destruct (Map_RES_Extra.P.F.eq_dec r r).
-      auto.
-      contradiction n.
-      auto.
-Qed.
 (** Let [WFG_of] be the definition of a finite WFG defined
     as a sequence of edges. *)
-Definition WFG_of wfg s := 
-  forall (e:(tid * tid)%type), List.In e wfg <-> TEdge s e.
-(** Given [build_wfg_spec] it is easy to show that we can
-    always obtain a finite WFG from a dependency state [d].*)
-Corollary wfg_of_total:
-  forall s:state, exists wfg, WFG_of wfg s.
+Definition WFG_of s wfg := 
+  forall (e:(tid * tid)), List.In e wfg <-> TEdge s e.
+
+(**
+  We use [deps_of_total] to convert a [state] into
+  [dependencies] and then use Theorem [DependencyState.wfg_of_total]
+  to obtain the target WFG.
+  *)
+Theorem wfg_of_total:
+  forall s:state, exists wfg, WFG_of s wfg.
 Proof.
   intros.
   unfold WFG_of.
   destruct (deps_of_total s) as (d, Hd).
-  exists (build_wfg d).
+  destruct (DependencyState.wfg_of_total d) as (wfg, Hwfg).
+  exists wfg.
   destruct e as (t, t').
-  rewrite build_wfg_spec.
-  rewrite tedge_spec.
-  destruct Hd as (Hw, Hi).
-  unfold W_of in *.
-  unfold I_of in *.
-  split; (
-    intros;
-    destruct H as (r, (w, i));
-    apply Hw in w;
-    apply Hi in i;
-    exists r;
-    intuition).
+  split.
+  - intros.
+    apply Hwfg in H.
+    destruct H as (r, (Hw, Hi)).
+    rewrite (wedge_eq_waits_for Hd) in Hw.
+    rewrite (iedge_eq_impedes Hd) in Hi.
+    apply tedge_spec.
+    exists r; intuition.
+  - intros.
+    apply Hwfg.
+    unfold WFGEdge.
+    inversion H.
+    subst; simpl in *.
+    exists b.
+    rewrite (wedge_eq_waits_for Hd).
+    rewrite (iedge_eq_impedes Hd).
+    intuition.
 Qed.
 
+(** * Completeness for totally deadlocked states *)
 Section TOTALLY_COMPLETE.
 Variable s:state.
 Variable w:t_walk.
 Variable wfg: list (tid * tid) % type.
-Variable wfg_spec: WFG_of wfg s.
+Variable wfg_spec: WFG_of s wfg.
 
 (** Any edge in a graph [wfg] is a [TEdge] (i.e., a WFG edge). *)
 Lemma totally_deadlocked_edge:
@@ -332,7 +248,9 @@ Qed.
 
 End TOTALLY_COMPLETE.
 
-Section Totally.
+(** * Completeness for deadlocked states *)
+
+Section DeadlockedStates.
 
 Variable s : state.
 Variable deadlocked_tasks : Map_TID.t prog.
@@ -404,13 +322,13 @@ Proof.
   - apply impedes_conv.
     assumption.
 Qed.
-End Totally.
+End DeadlockedStates.
 
-Section COMPLETE.
+Section Bootstrap.
 Variable s:state.
 Variable w:t_walk.
 Variable wfg: list (tid * tid).
-Variable wfg_spec: WFG_of wfg s.
+Variable wfg_spec: WFG_of s wfg.
 Variable is_deadlocked : Deadlocked s.
 
 (** We can construct a totally deadlocked
@@ -419,14 +337,14 @@ Let deadlocked_inv:
   exists s' wfg',
   TotallyDeadlocked s' /\
   wfg' <> nil /\
-  WFG_of wfg' s' /\ 
+  WFG_of s' wfg' /\ 
   subgraph wfg' wfg.
 Proof.
   intros.
   unfold Deadlocked in *.
   destruct is_deadlocked as (tm, (tm', (Hp, Hd))).
   exists (get_phasers s, tm).
-  assert (exists wfg', WFG_of wfg' (get_phasers s, tm)).
+  assert (exists wfg', WFG_of (get_phasers s, tm) wfg').
   apply wfg_of_total.
   destruct H as (wfg', Hwfg).
   exists wfg'.
@@ -449,7 +367,7 @@ Qed.
     a subgraph of the WFG of the deadlocked state, which implies
     that any cycle in the WFG of the totally deadlocked state is
     also in the deadlocked state. *)
-Theorem deadlocked_has_cycle:
+Lemma deadlocked_has_cycle:
   exists c, Core.Cycle (Edge wfg) c.
 Proof.
   intros.
@@ -486,7 +404,7 @@ Proof.
     assumption.
 Qed.
 
-End COMPLETE.
+End Bootstrap.
 
 (**
   The main theorem of completness uses [deadlocked_has_cycle]
